aneris/examples/crdt/statelib/resources/resources_global.v
@@ -10,7 +10,7 @@ From aneris.examples.crdt.statelib.STS Require Import lst gst utils.
 From iris.base_logic.lib Require Import invariants.
 
 From aneris.examples.crdt.statelib.resources
-  Require Import resources resources_inv resources_local.
+  Require Import utils resources_inv resources_local.
 
 Section AboutGlobal.
   Context `{CRDT_Op: Type,
