aneris/examples/crdt/statelib/resources/resources_local.v
@@ -10,7 +10,7 @@ From aneris.examples.crdt.statelib.STS Require Import lst gst utils.
 From iris.base_logic.lib Require Import invariants.
 
 From aneris.examples.crdt.statelib.resources
-  Require Import resources resources_inv.
+  Require Import utils resources_inv.
 
 
 
